Restore old wpcs for grove file ops

src/goose_lang/ffi/grove_ffi/typed_impl.v
@@ -87,7 +87,7 @@ Section grove.
       The Go implementation will accordingly abort the program if an I/O error occurs. *)
   Definition FileWrite : val :=
     λ: "f" "c",
-      let: "err" := ExternalOp FileWriteOp ("f", (Fst $ Fst "c", Snd $ Fst "c")) in
+      let: "err" := ExternalOp FileWriteOp ("f", (slice.ptr "c", slice.len "c")) in
       if: "err" then control.impl.Exit #() else
       #().
 
@@ -95,7 +95,7 @@ Section grove.
       The Go implementation will accordingly abort the program if an I/O error occurs. *)
   Definition FileAppend : val :=
     λ: "f" "c",
-      let: "err" := ExternalOp FileAppendOp ("f", (Fst $ Fst "c", Snd $ Fst "c")) in
+      let: "err" := ExternalOp FileAppendOp ("f", (slice.ptr "c", slice.len "c")) in
       if: "err" then control.impl.Exit #() else
       #().
 
